inductive_proof/Append-only_log/App.fst
@@ -1,8 +1,5 @@
 module App
 
-open FStar.Seq
-open FStar.Ghost
-
 #set-options "--query_stats"
 // the concrete state type
 // It is a sequence of pairs of timestamp and message.
@@ -41,23 +38,15 @@ let is_suffix_s (s l:concrete_st) : Tot prop =
 
 // apply an operation to a state
 let do (s:concrete_st) (op:op_t) : concrete_st =
-  cons (fst op) s
+  cons (fst op) s 
 
 let lem_do (a b:concrete_st) (op:op_t)
    : Lemma (requires eq a b)
            (ensures eq (do a op) (do b op)) = ()
            
 //conflict resolution
-let resolve_conflict (x:op_t) (y:op_t{fst x <> fst y}) : (l:log{(forall e. mem e l <==> (e == x \/ e == y))}) =
-  if lt (fst y) (fst x)
-    then cons y (cons x empty)
-      else cons x (cons y empty)
-
-let resolve_conflict_prop (x y:op_t)
-  : Lemma (requires fst x <> fst y)
-          (ensures (lt (fst y) (fst x) <==> last (resolve_conflict x y) = x) /\
-                   (last (resolve_conflict x y) <> x <==> lt (fst x) (fst y)))
-  = ()
+let resolve_conflict (x:op_t) (y:op_t{fst x <> fst y}) : resolve_conflict_res =
+  if lt (fst y) (fst x) then First else Second
 
 let rec union_s (l1 l2:concrete_st) 
   : Tot (u:concrete_st{forall e. mem e u <==> mem e l1 \/ mem e l2}) 
@@ -82,7 +71,8 @@ let diff_s (s1:concrete_st) (lca:concrete_st{is_suffix_s lca s1})
 let rec lem_foldl (s:concrete_st) (l:log)
   : Lemma (requires true)
           (ensures (length l = 0 ==> (apply_log s l = s)) /\
-                   (is_suffix_s s (apply_log s l)))
+                   (is_suffix_s s (apply_log s l)) /\
+                   (length l > 0 ==> length (apply_log s l) > length s))
           (decreases length l)
           [SMTPat (is_suffix_s s (apply_log s l))]
   = match length l with
@@ -97,7 +87,7 @@ let lem_foldl_forall (s:concrete_st)
 let concrete_merge (lca s1 s2:concrete_st) 
   : Pure concrete_st
          (requires (exists l1 l2. apply_log lca l1 == s1 /\ apply_log lca l2 == s2))
-         (ensures (fun _ -> True)) = 
+         (ensures (fun _ -> True)) =
   //lem_foldl_forall lca;
   let la = diff_s s1 lca in
   let lb = diff_s s2 lca in
@@ -149,10 +139,12 @@ let linearizable_s1_0''_ind (lca s1 s2':st) (last2:op_t)
           (ensures eq (do (v_of s2') last2) (concrete_merge (v_of lca) (v_of s1) (do (v_of s2') last2))) = ()
 
 let linearizable_s1_0_s2_0_base (lca s1 s2:st)
-  : Lemma (requires ops_of s1 == ops_of lca /\ ops_of s2 == ops_of lca)
+  : Lemma (requires (exists l1. v_of s1 == apply_log (v_of lca) l1) /\
+                    (exists l2. v_of s2 == apply_log (v_of lca) l2) /\
+                    ops_of s1 == ops_of lca /\ ops_of s2 == ops_of lca)
         
           (ensures eq (v_of lca) (concrete_merge (v_of lca) (v_of s1) (v_of s2))) = ()
-
+          
 let linearizable_s2_0''_base_base (lca s1' s2:st) (last1:op_t)
   : Lemma (requires consistent_branches lca s1' s2 /\
                     is_prefix (ops_of lca) (snoc (ops_of s1') last1) /\
@@ -203,7 +195,7 @@ let linearizable_gt0_base_last1 (lca s1 s2:st) (last1 last2:op_t)
                     fst last1 <> fst last2 /\ 
                     (exists l2. (do (v_of s2) last2 == apply_log (v_of lca) l2)) /\
                     (exists l1. (do (v_of s1) last1 == apply_log (v_of lca) l1)) /\
-                    last (resolve_conflict last1 last2) = last1)
+                    First? (resolve_conflict last1 last2))
          
           (ensures (eq (do (concrete_merge (v_of lca) (v_of s1) (do (v_of s2) last2)) last1)
                        (concrete_merge (v_of lca) (do (v_of s1) last1) (do (v_of s2) last2)))) =
@@ -221,7 +213,7 @@ let linearizable_gt0_base_last2 (lca s1 s2:st) (last1 last2:op_t)
                     fst last1 <> fst last2 /\ 
                     (exists l2. (do (v_of s2) last2 == apply_log (v_of lca) l2)) /\
                     (exists l1. (do (v_of s1) last1 == apply_log (v_of lca) l1)) /\
-                    last (resolve_conflict last1 last2) <> last1)
+                    Second? (resolve_conflict last1 last2))
          
           (ensures (eq (do (concrete_merge (v_of lca) (do (v_of s1) last1) (v_of s2)) last2)
                        (concrete_merge (v_of lca) (do (v_of s1) last1) (do (v_of s2) last2)))) =
@@ -240,20 +232,181 @@ let linearizable_gt0_base (lca s1 s2:st) (last1 last2:op_t)
                     (exists l2. (do (v_of s2) last2 == apply_log (v_of lca) l2)) /\
                     (exists l1. (do (v_of s1) last1 == apply_log (v_of lca) l1)))
          
-          (ensures (last (resolve_conflict last1 last2) = last1 ==>
+          (ensures (First? (resolve_conflict last1 last2) ==>
                       (eq (do (concrete_merge (v_of lca) (v_of s1) (do (v_of s2) last2)) last1)
                          (concrete_merge (v_of lca) (do (v_of s1) last1) (do (v_of s2) last2)))) /\
 
-                   (last (resolve_conflict last1 last2) <> last1 ==>
+                   (Second? (resolve_conflict last1 last2) ==>
                       (eq (do (concrete_merge (v_of lca) (do (v_of s1) last1) (v_of s2)) last2)
                          (concrete_merge (v_of lca) (do (v_of s1) last1) (do (v_of s2) last2))))) =
-  if last (resolve_conflict last1 last2) = last1 then
+  if First? (resolve_conflict last1 last2) then
     linearizable_gt0_base_last1 lca s1 s2 last1 last2
   else linearizable_gt0_base_last2 lca s1 s2 last1 last2
 
+(*let lem_diff (s1 l:log)
+  : Lemma (requires distinct_ops s1 /\ is_prefix l s1)
+          (ensures distinct_ops (diff s1 l) /\ (forall id. mem_id id (diff s1 l) <==> mem_id id s1 /\ not (mem_id id l)) /\
+                   (forall id. mem_id id s1 <==> mem_id id l \/ mem_id id (diff s1 l)) /\
+                   (Seq.length s1 > Seq.length l ==> (last s1 == last (diff s1 l) /\ Seq.length (diff s1 l) > 0) /\
+                     (let _, l1 = un_snoc s1 in
+                      let _, ld = un_snoc (diff s1 l) in
+                      l1 = ld) /\
+                     (let s1',lastop = un_snoc s1 in 
+                       diff s1' l == fst (un_snoc (diff s1 l)))))
+  = let s = snd (split s1 (length l)) in
+    lemma_split s1 (length l);
+    lemma_append_count_assoc_fst l s
+
+let rec split_prefix (s:concrete_st) (l:log) (a:log)
+  : Lemma (requires is_prefix l a)
+          (ensures (apply_log s a == apply_log (apply_log s l) (diff a l)) /\
+                   (forall e. mem e l ==> mem e a) /\
+                   (Seq.length a > Seq.length l ==> (last a) == (last (diff a l))))
+          (decreases Seq.length l)
+  = match Seq.length l with
+    |0 -> ()
+    |1 -> ()
+    |_ -> split_prefix (do s (head l)) (tail l) (tail a)*)
+
+let lem_diff_s (s1 l:concrete_st)
+  : Lemma (requires is_suffix_s l s1)
+          (ensures (Seq.length s1 > Seq.length l ==> (head s1 == head (diff_s s1 l) /\ Seq.length (diff_s s1 l) > 0) /\
+                     (let h1 = head s1 in
+                      let hd = head (diff_s s1 l) in
+                      h1 = hd) /\
+                     (let s1' = tail s1 in 
+                       is_suffix_s l s1' /\
+                       diff_s s1' l == tail (diff_s s1 l))))
+  = let s = fst (split s1 (length s1 - length l)) in
+    lemma_split s1 (length s1 - length l);
+    lemma_mem_append s l
+
+let lem_unionb (a b:concrete_st)
+  : Lemma (requires length a > 0 /\ length b > 0 /\
+                    head b > head a)
+          (ensures union_s a b == cons (head b) (union_s a (tail b))) = ()
+
+let lem_uniona (a b:concrete_st)
+  : Lemma (requires length a > 0 /\ length b > 0 /\
+                    head a > head b)
+          (ensures union_s a b == cons (head a) (union_s (tail a) b)) = ()
+
+#push-options "--z3rlimit 20"
+let linearizable_gt0_ind_c2 (lca s1 s2:st) (last1 last2:op_t)
+  : Lemma (requires consistent_branches_s2_gt0 lca s1 s2 /\
+                    fst last1 <> fst last2 /\
+                    distinct_ops (snoc (ops_of s1) last1) /\
+                    distinct_ops (snoc (ops_of s2) last2) /\
+                    (exists l1. (do (v_of s1) last1 == apply_log (v_of lca) l1)) /\
+                    (exists l2. (do (v_of s2) last2 == apply_log (v_of lca) l2)) /\
+                    ops_of s1 = ops_of lca /\
+                    Second? (resolve_conflict last1 last2) /\
+                    (//let s2' = inverse_st s2 in
+                  //  (exists l2. (do (v_of s2') last2 == apply_log (v_of lca) l2)) /\
+                   // (exists l2. (v_of s2' == apply_log (v_of lca) l2)) /\
+                  //  (exists l1. (v_of s1 == apply_log (v_of lca) l1)) /\
+                    (exists l2. (v_of s2 == apply_log (v_of lca) l2))
+                    (*consistent_branches lca s1 s2' /\
+                    eq (do (concrete_merge (v_of lca) (do (v_of s1) last1) (v_of s2')) last2)
+                       (concrete_merge (v_of lca) (do (v_of s1) last1) (do (v_of s2') last2)*)))
+       
+          (ensures eq (do (concrete_merge (v_of lca) (do (v_of s1) last1) (v_of s2)) last2)
+                      (concrete_merge (v_of lca) (do (v_of s1) last1) (do (v_of s2) last2)))
+          [SMTPat (eq (do (concrete_merge (v_of lca) (do (v_of s1) last1) (v_of s2)) last2)
+                      (concrete_merge (v_of lca) (do (v_of s1) last1) (do (v_of s2) last2)))] = 
+  assert (fst last2 > fst last1); 
+  let s1v = do (v_of s1) last1 in
+  let s2v = do (v_of s2) last2 in
+  let da = (diff_s s1v (v_of lca)) in
+  let db = (diff_s s2v (v_of lca)) in
+  let db' = (diff_s (v_of s2) (v_of lca)) in
+  let s1op = (snoc (ops_of s1) last1) in
+  let s2op = (snoc (ops_of s2) last2) in
+  lem_diff s1op (ops_of lca);
+  split_prefix init_st (ops_of lca) s1op;
+  lem_foldl (v_of lca) (diff s1op (ops_of lca));
+  assert (length da > 0);
+  lem_diff s2op (ops_of lca);
+  split_prefix init_st (ops_of lca) s2op;
+  lem_foldl (v_of lca) (diff s2op (ops_of lca));
+  assert (length db > 0);
+  
+  assert (s1v == cons (fst last1) (v_of s1));
+  assert (s2v == cons (fst last2) (v_of s2));
+  lemma_tl (fst last2) (v_of s2);
+  assert (v_of s2 == tail s2v);
+  assert (concrete_merge (v_of lca) s1v s2v == Seq.append (union_s da db) (v_of lca)); 
+  lem_diff_s s2v (v_of lca);
+  assert (head db = fst last2); 
+  lem_diff_s s1v (v_of lca);
+  assert (head da = fst last1); 
+  assert (head db > head da); 
+  lem_unionb da db; 
+  assert (union_s da db == cons (fst last2) (union_s da db')); 
+  assert (do (concrete_merge (v_of lca) s1v (v_of s2)) last2 ==
+          cons (fst last2) (Seq.append (union_s da db') (v_of lca)));
+  append_assoc (create 1 (fst last2)) (union_s da db') (v_of lca)
+
+#push-options "--z3rlimit 100"
+let linearizable_gt0_ind_c1 (lca s1 s2:st) (last1 last2:op_t)
+  : Lemma (requires consistent_branches_s2_gt0 lca s1 s2 /\
+                    fst last1 <> fst last2 /\
+                    distinct_ops (snoc (ops_of s1) last1) /\
+                    distinct_ops (snoc (ops_of s2) last2) /\
+                    (exists l1. (do (v_of s1) last1 == apply_log (v_of lca) l1)) /\
+                    (exists l2. (do (v_of s2) last2 == apply_log (v_of lca) l2)) /\
+                    First? (resolve_conflict last1 last2) /\
+                    (let s2' = inverse_st s2 in
+                    (exists l2. (do (v_of s2') last2 == apply_log (v_of lca) l2)) /\
+                    (exists l2. (v_of s2' == apply_log (v_of lca) l2)) /\
+                    (exists l1. (v_of s1 == apply_log (v_of lca) l1)) /\
+                    (exists l2. (v_of s2 == apply_log (v_of lca) l2)) /\
+                    (consistent_branches lca s1 s2' /\
+                    eq (do (concrete_merge (v_of lca) (v_of s1) (do (v_of s2') last2)) last1)
+                       (concrete_merge (v_of lca) (do (v_of s1) last1) (do (v_of s2') last2)))))
+       
+          (ensures eq (do (concrete_merge (v_of lca) (v_of s1) (do (v_of s2) last2)) last1)
+                      (concrete_merge (v_of lca) (do (v_of s1) last1) (do (v_of s2) last2)))
+          [SMTPat (eq (do (concrete_merge (v_of lca) (v_of s1) (do (v_of s2) last2)) last1)
+                      (concrete_merge (v_of lca) (do (v_of s1) last1) (do (v_of s2) last2)))] = 
+  assert (fst last1 > fst last2); 
+  let s1v = do (v_of s1) last1 in
+  let s2v = do (v_of s2) last2 in
+  let da = (diff_s s1v (v_of lca)) in
+  let db = (diff_s s2v (v_of lca)) in
+  let da' = (diff_s (v_of s1) (v_of lca)) in
+  let s1op = (snoc (ops_of s1) last1) in
+  let s2op = (snoc (ops_of s2) last2) in
+  lem_diff s2op (ops_of lca); 
+  split_prefix init_st (ops_of lca) s2op;
+  lem_foldl (v_of lca) (diff s2op (ops_of lca));
+  assert (length db > 0);
+  lem_diff s1op (ops_of lca);
+  split_prefix init_st (ops_of lca) s1op;
+  lem_foldl (v_of lca) (diff s1op (ops_of lca));
+  assert (length da > 0); 
+  
+  assert (s1v == cons (fst last1) (v_of s1));
+  assert (s2v == cons (fst last2) (v_of s2));
+  lemma_tl (fst last1) (v_of s1);
+  assert (v_of s1 == tail s1v);
+  assert (concrete_merge (v_of lca) s1v s2v == Seq.append (union_s da db) (v_of lca)); 
+  lem_diff_s s2v (v_of lca);
+  assert (head db = fst last2); 
+  lem_diff_s s1v (v_of lca);
+  assert (head da = fst last1); 
+  assert (head da > head db); 
+  lem_uniona da db; 
+  assert (union_s da db == cons (fst last1) (union_s da' db)); 
+  assert (do (concrete_merge (v_of lca) (v_of s1) s2v) last1 ==
+          cons (fst last1) (Seq.append (union_s da' db) (v_of lca)));
+  append_assoc (create 1 (fst last1)) (union_s da' db) (v_of lca)
+                        
 let linearizable_gt0_ind (lca s1 s2:st) (last1 last2:op_t)
   : Lemma (requires consistent_branches_s2_gt0 lca s1 s2 /\
                     fst last1 <> fst last2 /\
+                    distinct_ops (snoc (ops_of s1) last1) /\
+                    distinct_ops (snoc (ops_of s2) last2) /\ 
                     (exists l1. (do (v_of s1) last1 == apply_log (v_of lca) l1)) /\
                     (exists l2. (do (v_of s2) last2 == apply_log (v_of lca) l2)) /\
                     (let s2' = inverse_st s2 in
@@ -264,22 +417,132 @@ let linearizable_gt0_ind (lca s1 s2:st) (last1 last2:op_t)
                     consistent_branches lca s1 s2'))
        
           (ensures (let s2' = inverse_st s2 in
-                   ((last (resolve_conflict last1 last2) = last1 /\
+                   ((First? (resolve_conflict last1 last2) /\
                     eq (do (concrete_merge (v_of lca) (v_of s1) (do (v_of s2') last2)) last1)
                        (concrete_merge (v_of lca) (do (v_of s1) last1) (do (v_of s2') last2))) ==>
                     (eq (do (concrete_merge (v_of lca) (v_of s1) (do (v_of s2) last2)) last1)
                         (concrete_merge (v_of lca) (do (v_of s1) last1) (do (v_of s2) last2)))) /\
                           
                    ((ops_of s1 = ops_of lca /\
-                    last (resolve_conflict last1 last2) <> last1 /\
+                    Second? (resolve_conflict last1 last2) /\
                     eq (do (concrete_merge (v_of lca) (do (v_of s1) last1) (v_of s2')) last2)
                        (concrete_merge (v_of lca) (do (v_of s1) last1) (do (v_of s2') last2))) ==>
                     (eq (do (concrete_merge (v_of lca) (do (v_of s1) last1) (v_of s2)) last2)
-                        (concrete_merge (v_of lca) (do (v_of s1) last1) (do (v_of s2) last2)))))) = admit()
+                        (concrete_merge (v_of lca) (do (v_of s1) last1) (do (v_of s2) last2)))))) = ()
+  
+let linearizable_gt0_ind1_c2 (lca s1 s2:st) (last1 last2:op_t)
+  : Lemma (requires consistent_branches_s1_gt0 lca s1 s2 /\
+                    fst last1 <> fst last2 /\
+                    distinct_ops (snoc (ops_of s1) last1) /\
+                    distinct_ops (snoc (ops_of s2) last2) /\ 
+                    (exists l1. (do (v_of s1) last1 == apply_log (v_of lca) l1)) /\
+                    (exists l2. (do (v_of s2) last2 == apply_log (v_of lca) l2)) /\
+                    Second? (resolve_conflict last1 last2) /\
+                    (let s1' = inverse_st s1 in
+                    (exists l1. (do (v_of s1') last1 == apply_log (v_of lca) l1)) /\
+                    (exists l1. (v_of s1' == apply_log (v_of lca) l1)) /\
+                    (exists l1. (v_of s1 == apply_log (v_of lca) l1)) /\
+                    (exists l2. (v_of s2 == apply_log (v_of lca) l2)) /\
+                    consistent_branches lca s1' s2 /\
+                    eq (do (concrete_merge (v_of lca) (do (v_of s1') last1) (v_of s2)) last2)
+                       (concrete_merge (v_of lca) (do (v_of s1') last1) (do (v_of s2) last2))))
+        
+          (ensures eq (do (concrete_merge (v_of lca) (do (v_of s1) last1) (v_of s2)) last2)
+                       (concrete_merge (v_of lca) (do (v_of s1) last1) (do (v_of s2) last2))) 
+          [SMTPat (eq (do (concrete_merge (v_of lca) (do (v_of s1) last1) (v_of s2)) last2)
+                      (concrete_merge (v_of lca) (do (v_of s1) last1) (do (v_of s2) last2)))] =
+  assert (fst last2 > fst last1); 
+  let s1v = do (v_of s1) last1 in
+  let s2v = do (v_of s2) last2 in
+  let da = (diff_s s1v (v_of lca)) in
+  let db = (diff_s s2v (v_of lca)) in
+  let db' = (diff_s (v_of s2) (v_of lca)) in
+  let s1op = (snoc (ops_of s1) last1) in
+  let s2op = (snoc (ops_of s2) last2) in
+  split_prefix init_st (ops_of lca) s1op;
+  lem_foldl (v_of lca) (diff s1op (ops_of lca));
+  assert (length da > 0);
+  lem_diff s2op (ops_of lca);
+  split_prefix init_st (ops_of lca) s2op;
+  lem_foldl (v_of lca) (diff s2op (ops_of lca));
+  assert (length db > 0);
+  
+  assert (s1v == cons (fst last1) (v_of s1));
+  assert (s2v == cons (fst last2) (v_of s2));
+  lemma_tl (fst last2) (v_of s2);
+  assert (v_of s2 == tail s2v); 
+  assert (concrete_merge (v_of lca) s1v s2v == Seq.append (union_s da db) (v_of lca)); 
+  lem_diff_s s2v (v_of lca);
+  assert (head db = fst last2); 
+  lem_diff_s s1v (v_of lca);
+  assert (head da = fst last1); 
+  assert (head db > head da); 
+  lem_unionb da db; 
+  assert (union_s da db == cons (fst last2) (union_s da db')); 
+  assert (do (concrete_merge (v_of lca) s1v (v_of s2)) last2 ==
+          cons (fst last2) (Seq.append (union_s da db') (v_of lca)));
+  append_assoc (create 1 (fst last2)) (union_s da db') (v_of lca)
 
+let linearizable_gt0_ind1_c1 (lca s1 s2:st) (last1 last2:op_t)
+  : Lemma (requires consistent_branches_s1_gt0 lca s1 s2 /\
+                    fst last1 <> fst last2 /\
+                    distinct_ops (snoc (ops_of s1) last1) /\
+                    distinct_ops (snoc (ops_of s2) last2) /\ 
+                    (exists l1. (do (v_of s1) last1 == apply_log (v_of lca) l1)) /\
+                    (exists l2. (do (v_of s2) last2 == apply_log (v_of lca) l2)) /\
+                    ops_of s2 = ops_of lca /\
+                    First? (resolve_conflict last1 last2) /\
+                    (//let s1' = inverse_st s1 in
+                   // (exists l1. (do (v_of s1') last1 == apply_log (v_of lca) l1)) /\
+                   // (exists l1. (v_of s1' == apply_log (v_of lca) l1)) /\
+                    (exists l1. (v_of s1 == apply_log (v_of lca) l1)) 
+                   // (exists l2. (v_of s2 == apply_log (v_of lca) l2)) /\
+                    (*consistent_branches lca s1' s2 /\
+                    eq (do (concrete_merge (v_of lca) (v_of s1') (do (v_of s2) last2)) last1)
+                       (concrete_merge (v_of lca) (do (v_of s1') last1) (do (v_of s2) last2)*)))
+        
+          (ensures eq (do (concrete_merge (v_of lca) (v_of s1) (do (v_of s2) last2)) last1)
+                      (concrete_merge (v_of lca) (do (v_of s1) last1) (do (v_of s2) last2)))
+          [SMTPat (eq (do (concrete_merge (v_of lca) (v_of s1) (do (v_of s2) last2)) last1)
+                      (concrete_merge (v_of lca) (do (v_of s1) last1) (do (v_of s2) last2)))] = 
+  assert (fst last1 > fst last2); 
+  let s1v = do (v_of s1) last1 in
+  let s2v = do (v_of s2) last2 in
+  let da = (diff_s s1v (v_of lca)) in
+  let db = (diff_s s2v (v_of lca)) in
+  let da' = (diff_s (v_of s1) (v_of lca)) in
+  let s1op = (snoc (ops_of s1) last1) in
+  let s2op = (snoc (ops_of s2) last2) in
+  lem_diff s2op (ops_of lca); 
+  split_prefix init_st (ops_of lca) s2op;
+  lem_foldl (v_of lca) (diff s2op (ops_of lca));
+  assert (length db > 0); 
+  lem_diff s1op (ops_of lca);
+  split_prefix init_st (ops_of lca) s1op;
+  lem_foldl (v_of lca) (diff s1op (ops_of lca));
+  assert (length da > 0);
+   
+  assert (s1v == cons (fst last1) (v_of s1));
+  assert (s2v == cons (fst last2) (v_of s2));
+  lemma_tl (fst last1) (v_of s1);
+  assert (v_of s1 == tail s1v);
+  assert (concrete_merge (v_of lca) s1v s2v == Seq.append (union_s da db) (v_of lca)); 
+  lem_diff_s s2v (v_of lca);
+  assert (head db = fst last2); 
+  lem_diff_s s1v (v_of lca);
+  assert (head da = fst last1); 
+  assert (head da > head db); 
+  lem_uniona da db; 
+  assert (union_s da db == cons (fst last1) (union_s da' db)); 
+  assert (do (concrete_merge (v_of lca) (v_of s1) s2v) last1 ==
+          cons (fst last1) (Seq.append (union_s da' db) (v_of lca)));
+  append_assoc (create 1 (fst last1)) (union_s da' db) (v_of lca)
+                       
 let linearizable_gt0_ind1 (lca s1 s2:st) (last1 last2:op_t)
   : Lemma (requires consistent_branches_s1_gt0 lca s1 s2 /\
                     fst last1 <> fst last2 /\
+                    distinct_ops (snoc (ops_of s1) last1) /\
+                    distinct_ops (snoc (ops_of s2) last2) /\ 
                     (exists l1. (do (v_of s1) last1 == apply_log (v_of lca) l1)) /\
                     (exists l2. (do (v_of s2) last2 == apply_log (v_of lca) l2)) /\
                     (let s1' = inverse_st s1 in
@@ -291,17 +554,17 @@ let linearizable_gt0_ind1 (lca s1 s2:st) (last1 last2:op_t)
         
           (ensures (let s1' = inverse_st s1 in
                    ((ops_of s2 = ops_of lca /\
-                   last (resolve_conflict last1 last2) = last1 /\
+                   First? (resolve_conflict last1 last2) /\
                    eq (do (concrete_merge (v_of lca) (v_of s1') (do (v_of s2) last2)) last1)
                       (concrete_merge (v_of lca) (do (v_of s1') last1) (do (v_of s2) last2))) ==>
                    eq (do (concrete_merge (v_of lca) (v_of s1) (do (v_of s2) last2)) last1)
                       (concrete_merge (v_of lca) (do (v_of s1) last1) (do (v_of s2) last2))) /\
 
-                   ((last (resolve_conflict last1 last2) <> last1 /\
+                   ((Second? (resolve_conflict last1 last2) /\
                     eq (do (concrete_merge (v_of lca) (do (v_of s1') last1) (v_of s2)) last2)
                        (concrete_merge (v_of lca) (do (v_of s1') last1) (do (v_of s2) last2)) ==>
                     eq (do (concrete_merge (v_of lca) (do (v_of s1) last1) (v_of s2)) last2)
-                       (concrete_merge (v_of lca) (do (v_of s1) last1) (do (v_of s2) last2)))))) = admit()
+                       (concrete_merge (v_of lca) (do (v_of s1) last1) (do (v_of s2) last2)))))) = ()
 
 ////////////////////////////////////////////////////////////////
 //// Sequential implementation //////
@@ -329,3 +592,126 @@ let do_eq (st_s:concrete_st_s) (st:concrete_st) (op:op_t)
   = ()
 
 ////////////////////////////////////////////////////////////////
+
+(*let unique_st (s:concrete_st) = forall e.{:pattern count e s} count e s <= 1
+
+let concrete_st_u = s:concrete_st{unique_st s} 
+
+let distinct_append (a b:concrete_st)
+  : Lemma (requires unique_st a /\ unique_st b /\
+                    (forall e. mem e a ==> not (mem e b)))
+          (ensures (unique_st (Seq.append a b)) /\
+                   (forall e. mem e (Seq.append a b) <==> mem e a \/ mem e b)) =
+  lemma_append_count a b
+  
+let rec apply_unique_st (s:concrete_st_u) (l:log)
+  : Lemma (requires distinct_ops l /\ (forall id. mem_id id l ==> not (mem id s)))
+          (ensures unique_st (apply_log s l))
+          (decreases length l) =
+  match length l with
+  |0 -> ()
+  |_ -> distinct_append (create 1 (fst (head l))) s;
+       assert (unique_st (do s (head l)));
+       mem_cons (fst (head l)) s; // (forall e. mem e (do s (head l)) ==> not (mem_id e (tail l)));
+       mem_cons (head l) (tail l);
+       distinct_invert_append (create 1 (head l)) (tail l); // distinct_ops (tail l)
+       apply_unique_st (do s (head l)) (tail l)
+
+let st_is_unique (lca:st) 
+  : Lemma (ensures unique_st (v_of lca)) =
+  apply_unique_st init_st (ops_of lca)*)
+
+(*
+#push-options "--z3rlimit 20"
+let linearizable_gt0_s2 (lca s1 s2:st)
+  : Lemma (requires consistent_branches_s1s2_gt0 lca s1 s2 /\
+                    (let _, last1 = un_snoc (ops_of s1) in
+                    let _, last2 = un_snoc (ops_of s2) in
+                    fst last1 <> fst last2 /\
+                    Second? (resolve_conflict last1 last2) /\
+                    (exists l2. (v_of (inverse_st s2) == apply_log (v_of lca) l2)) /\
+                    (exists l2. (v_of s2) == apply_log (v_of lca) l2) /\
+                    (exists l1. (v_of s1) == apply_log (v_of lca) l1)))
+          (ensures (let pre2, last2 = un_snoc (ops_of s2) in                   
+                   eq (do (concrete_merge (v_of lca) (v_of s1) (v_of (inverse_st s2))) last2)
+                      (concrete_merge (v_of lca) (v_of s1) (v_of s2)))) = 
+  let _, last1 = un_snoc (ops_of s1) in
+  let _, last2 = un_snoc (ops_of s2) in
+  assert (fst last2 > fst last1);
+  let s1' = inverse_st s1 in
+  let s2' = inverse_st s2 in
+  let da = (diff_s (v_of s1) (v_of lca)) in
+  let db = (diff_s (v_of s2) (v_of lca)) in
+  let db' = (diff_s (v_of s2') (v_of lca)) in
+  lem_diff (ops_of s1) (ops_of lca);
+  split_prefix init_st (ops_of lca) (ops_of s1);
+  lem_foldl (v_of lca) (diff (ops_of s1) (ops_of lca));
+  assert (length (diff_s (v_of s1) (v_of lca)) > 0);
+  lem_diff (ops_of s2) (ops_of lca);
+  split_prefix init_st (ops_of lca) (ops_of s2);
+  lem_foldl (v_of lca) (diff (ops_of s2) (ops_of lca));
+  assert (length (diff_s (v_of s2) (v_of lca)) > 0); 
+  assert (v_of s1 == cons (fst last1) (v_of s1'));
+  assert (v_of s2 == cons (fst last2) (v_of s2'));
+  lemma_tl (fst last2) (v_of s2');
+  assert (v_of s2' == tail (v_of s2)); 
+  assert (concrete_merge (v_of lca) (v_of s1) (v_of s2) ==
+          Seq.append (union_s da db) (v_of lca)); 
+  lem_diff_s (v_of s2) (v_of lca);
+  assert (head db = fst last2); 
+  lem_diff_s (v_of s1) (v_of lca);
+  assert (head da = fst last1); 
+  assert (head db > head da); 
+  lem_unionb da db; 
+  assert (union_s da db == cons (fst last2) (union_s da db')); 
+  assert (do (concrete_merge (v_of lca) (v_of s1) (v_of (inverse_st s2))) last2 ==
+          cons (fst last2) (Seq.append (union_s da db') (v_of lca)));
+  append_assoc (create 1 (fst last2)) (union_s da db') (v_of lca)
+
+let linearizable_gt0_s1 (lca s1 s2:st)
+  : Lemma (requires consistent_branches_s1s2_gt0 lca s1 s2 /\
+                    (let _, last1 = un_snoc (ops_of s1) in
+                    let _, last2 = un_snoc (ops_of s2) in
+                    fst last1 <> fst last2 /\
+                    First? (resolve_conflict last1 last2) /\
+                    (exists l1. (v_of (inverse_st s1) == apply_log (v_of lca) l1)) /\
+                    (exists l2. (v_of s2) == apply_log (v_of lca) l2) /\
+                    (exists l1. (v_of s1) == apply_log (v_of lca) l1)))
+          (ensures (let _, last1 = un_snoc (ops_of s1) in
+                   eq (do (concrete_merge (v_of lca) (v_of (inverse_st s1)) (v_of s2)) last1)
+                      (concrete_merge (v_of lca) (v_of s1) (v_of s2)))) = 
+  let _, last1 = un_snoc (ops_of s1) in
+  let _, last2 = un_snoc (ops_of s2) in
+  assert (fst last1 > fst last2);
+  let s1' = inverse_st s1 in
+  let s2' = inverse_st s2 in
+  let da = (diff_s (v_of s1) (v_of lca)) in
+  let db = (diff_s (v_of s2) (v_of lca)) in
+  let da' = (diff_s (v_of s1') (v_of lca)) in
+  lem_diff (ops_of s1) (ops_of lca);
+  split_prefix init_st (ops_of lca) (ops_of s1);
+  lem_foldl (v_of lca) (diff (ops_of s1) (ops_of lca));
+  assert (length (diff_s (v_of s1) (v_of lca)) > 0);
+  lem_diff (ops_of s2) (ops_of lca);
+  split_prefix init_st (ops_of lca) (ops_of s2);
+  lem_foldl (v_of lca) (diff (ops_of s2) (ops_of lca));
+  assert (length (diff_s (v_of s2) (v_of lca)) > 0); 
+  assert (v_of s1 == cons (fst last1) (v_of s1'));
+  assert (v_of s2 == cons (fst last2) (v_of s2'));
+  lemma_tl (fst last1) (v_of s1');
+  assert (v_of s1' == tail (v_of s1)); 
+  assert (concrete_merge (v_of lca) (v_of s1) (v_of s2) ==
+          Seq.append (union_s da db) (v_of lca)); 
+  lem_diff_s (v_of s2) (v_of lca);
+  assert (head db = fst last2); 
+  lem_diff_s (v_of s1) (v_of lca);
+  assert (head da = fst last1); 
+  assert (head db < head da); 
+  lem_uniona da db; 
+  assert (union_s da db == cons (fst last1) (union_s da' db)); 
+  assert (do (concrete_merge (v_of lca) (v_of (inverse_st s1)) (v_of s2)) last1 ==
+          cons (fst last1) (Seq.append (union_s da' db) (v_of lca)));
+  append_assoc (create 1 (fst last1)) (union_s da' db) (v_of lca)
+#pop-options
+
+*)
