inductive_proof/SeqUtils.fst
@@ -2,6 +2,8 @@ module SeqUtils
 
 open FStar.Seq
 
+let lt (a b:pos) : bool = a < b
+
 type seq_assoc (a:eqtype) (b:Type) = seq (a & b)
 
 let rec count_assoc_fst (#a:eqtype) (#b:Type) (id:a) (l:seq_assoc a b)
@@ -44,6 +46,13 @@ let distinct_invert_append (#t1:eqtype) (#t2:Type) (a b:seq_assoc t1 t2)
       //[SMTPat (distinct_assoc_fst (a ++ b))]
   = lemma_append_count_assoc_fst a b
 
+let distinct_append (#t1:eqtype) (#t2:Type) (a b:seq_assoc t1 t2)
+  : Lemma (requires distinct_assoc_fst a /\ distinct_assoc_fst b /\
+                    (forall id. mem_assoc_fst id a ==> not (mem_assoc_fst id b)))
+          (ensures (distinct_assoc_fst (a ++ b)) /\
+                   (forall id. mem_assoc_fst id (a ++ b) <==> mem_assoc_fst id a \/ mem_assoc_fst id b)) =
+  lemma_append_count_assoc_fst a b
+  
 // p is a prefix of l
 let is_prefix (#a:Type) (p l:Seq.seq a) =
   Seq.length l >= Seq.length p /\ Seq.equal p (Seq.slice l 0 (Seq.length p))
@@ -67,3 +76,131 @@ let lem_inverse (#a:eqtype) (lca s1:Seq.seq a)
                     Seq.length s1 > Seq.length lca)
           (ensures (is_prefix lca (fst (un_snoc s1)))) 
   = lemma_split (fst (un_snoc s1)) (length lca)
+
+let rec mem_ele_id (#t1 #t2:eqtype) (op:(t1 & t2)) (l:seq_assoc t1 t2)
+  : Lemma (requires mem op l)
+          (ensures mem_assoc_fst (fst op) l) (decreases length l) =
+  if head l = op then ()
+    else mem_ele_id op (tail l)
+    
+let rec lem_un_snoc_id (#t1 #t2:eqtype) (a b:seq_assoc t1 t2)
+  : Lemma (requires length b > 0 /\ a == fst (un_snoc b))
+          (ensures (forall id. mem_assoc_fst id a ==> mem_assoc_fst id b)) (decreases length a) =
+  match length a with
+  |0 -> ()
+  |_ -> lem_un_snoc_id (tail a) (tail b)
+
+let lem_diff (#t1 #t2:eqtype) (s1 l:seq_assoc t1 t2)
+  : Lemma (requires distinct_assoc_fst s1 /\ is_prefix l s1)
+          (ensures distinct_assoc_fst (diff s1 l) /\ 
+                   (forall id. mem_assoc_fst id (diff s1 l) <==> mem_assoc_fst id s1 /\ not (mem_assoc_fst id l)) /\
+                   (forall id. mem_assoc_fst id s1 <==> mem_assoc_fst id l \/ mem_assoc_fst id (diff s1 l)) /\
+                   (Seq.length s1 > Seq.length l ==> (last s1 == last (diff s1 l) /\ Seq.length (diff s1 l) > 0) /\
+                     (let _, l1 = un_snoc s1 in
+                      let _, ld = un_snoc (diff s1 l) in
+                      l1 = ld) /\
+                     (let s1',lastop = un_snoc s1 in 
+                       diff s1' l == fst (un_snoc (diff s1 l)))))
+  = let s = snd (split s1 (length l)) in
+    lemma_split s1 (length l);
+    lemma_append_count_assoc_fst l s
+    
+let lem_diff_lastop (#t1 #t2:eqtype) (s1 l:seq_assoc t1 t2)
+  : Lemma (requires distinct_assoc_fst s1 /\ is_prefix l s1 /\ length s1 > length l)
+          (ensures (let s1',lastop = un_snoc s1 in 
+                    mem_assoc_fst (fst lastop) (diff s1 l))) =
+  lem_diff s1 l;
+  let ds1',lastop = un_snoc (diff s1 l) in 
+  lemma_mem_append ds1' (create 1 lastop);
+  mem_ele_id lastop (diff s1 l)
+
+let un_snoc_prop (#t1 #t2:eqtype) (a:seq_assoc t1 t2)
+  : Lemma (requires distinct_assoc_fst a /\ length a > 0)
+          (ensures (forall id. mem_assoc_fst id a <==> mem_assoc_fst id (fst (un_snoc a)) \/ id == fst (last a)) /\
+                   (forall id. mem_assoc_fst id a /\ id <> fst (last a) <==> mem_assoc_fst id (fst (un_snoc a))) /\
+                   (let _, l = un_snoc a in 
+                    mem_assoc_fst (fst l) a) /\ distinct_assoc_fst (fst (un_snoc a))) =
+  let p, l = un_snoc a in
+  lemma_split a (length a - 1);
+  lemma_append_count_assoc_fst p (snd (split a (length a - 1)));
+  distinct_invert_append p (snd (split a (length a - 1)))
+  
+let lem_lt_lastop_id_lca (#t2:eqtype) (lca s1:seq_assoc pos t2)
+  : Lemma (requires is_prefix lca s1 /\ length (diff s1 lca) > 0 /\ distinct_assoc_fst s1 /\
+                    (forall id id1. mem_assoc_fst id lca /\ mem_assoc_fst id1 (diff s1 lca) ==> lt id id1))
+          (ensures (let _, lastop = un_snoc s1 in
+                    (forall id. mem_assoc_fst id lca ==> lt id (fst lastop)))) =
+    distinct_invert_append lca (diff s1 lca); 
+    let pre, lst = un_snoc s1 in
+    lem_diff s1 lca;
+    mem_ele_id lst (diff s1 lca)
+
+let lastop_diff (#t2:eqtype) (l a:seq_assoc pos t2)
+  : Lemma (requires distinct_assoc_fst l /\ distinct_assoc_fst a /\ is_prefix l a /\
+                    (forall id id1. mem_assoc_fst id l /\ mem_assoc_fst id1 (diff a l) ==> lt id id1) /\
+                    length a > length l)
+          (ensures (length (diff a l) > 0) /\
+                   (let p, last = un_snoc a in
+                   mem_assoc_fst (fst last) a /\ mem_assoc_fst (fst last) (diff a l) /\
+                   (forall id id1. mem_assoc_fst id l /\ mem_assoc_fst id1 (diff p l) ==> lt id id1)))
+  = un_snoc_prop a;
+    lem_diff a l;
+    un_snoc_prop (diff a l);
+    lem_inverse l a
+
+let inverse_diff_id_s1' (#t2:eqtype) (l a b:seq_assoc pos t2)
+  : Lemma (requires distinct_assoc_fst l /\ distinct_assoc_fst a /\ distinct_assoc_fst b /\
+                    is_prefix l a /\ is_prefix l b /\
+                    length a > length l /\ 
+                    (forall id id1. mem_assoc_fst id l /\ mem_assoc_fst id1 (diff a l) ==> lt id id1) /\
+                    (forall id id1. mem_assoc_fst id l /\ mem_assoc_fst id1 (diff b l) ==> lt id id1) /\
+                    (forall id. mem_assoc_fst id (diff a l) ==> not (mem_assoc_fst id (diff b l))))
+          (ensures (forall id. mem_assoc_fst id (diff (fst (un_snoc a)) l) ==> not (mem_assoc_fst id (diff b l))))
+  = un_snoc_prop a;
+    lem_diff a l; 
+    lem_inverse l a;
+    lem_diff (fst (un_snoc a)) l
+
+let inverse_diff_id_s2' (#t2:eqtype) (l a b:seq_assoc pos t2)
+  : Lemma (requires distinct_assoc_fst l /\ distinct_assoc_fst a /\ distinct_assoc_fst b /\
+                    is_prefix l a /\ is_prefix l b /\
+                    length b > length l /\
+                    (forall id id1. mem_assoc_fst id l /\ mem_assoc_fst id1 (diff a l) ==> lt id id1) /\
+                    (forall id id1. mem_assoc_fst id l /\ mem_assoc_fst id1 (diff b l) ==> lt id id1) /\
+                    (forall id. mem_assoc_fst id (diff a l) ==> not (mem_assoc_fst id (diff b l))))
+          (ensures (forall id. mem_assoc_fst id (diff a l) ==> not (mem_assoc_fst id (diff (fst (un_snoc b)) l))))
+  = un_snoc_prop b;
+    lem_diff b l; 
+    lem_inverse l b;
+    lem_diff (fst (un_snoc b)) l
+
+let inverse_diff_id_s1'_s2' (#t2:eqtype) (l a b:seq_assoc pos t2)
+  : Lemma (requires distinct_assoc_fst l /\ distinct_assoc_fst a /\ distinct_assoc_fst b /\
+                    is_prefix l a /\ is_prefix l b /\
+                    length a > length l /\ length b > length l /\
+                    (forall id id1. mem_assoc_fst id l /\ mem_assoc_fst id1 (diff a l) ==> lt id id1) /\
+                    (forall id id1. mem_assoc_fst id l /\ mem_assoc_fst id1 (diff b l) ==> lt id id1) /\
+                    (forall id. mem_assoc_fst id (diff a l) ==> not (mem_assoc_fst id (diff b l))))
+          (ensures (forall id. mem_assoc_fst id (diff (fst (un_snoc a)) l) ==> not (mem_assoc_fst id (diff (fst (un_snoc b)) l))))
+  = un_snoc_prop a;
+    lem_diff a l; 
+    lem_inverse l a;
+    lem_diff (fst (un_snoc a)) l;
+    un_snoc_prop b;
+    lem_diff b l; 
+    lem_inverse l b;
+    lem_diff (fst (un_snoc b)) l
+    
+let lastop_neq (#t2:eqtype) (l a b:seq_assoc pos t2)
+  : Lemma (requires distinct_assoc_fst l /\ distinct_assoc_fst a /\ distinct_assoc_fst b /\
+                    is_prefix l a /\ is_prefix l b /\
+                    length a > length l /\ length b > length l /\
+                    (forall id id1. mem_assoc_fst id l /\ mem_assoc_fst id1 (diff a l) ==> lt id id1) /\
+                    (forall id id1. mem_assoc_fst id l /\ mem_assoc_fst id1 (diff b l) ==> lt id id1) /\
+                    (forall id. mem_assoc_fst id (diff a l) ==> not (mem_assoc_fst id (diff b l))))
+          (ensures (let p, la = un_snoc a in
+                    let _, lb = un_snoc b in
+                    fst la <> fst lb)) =
+  lastop_diff l a;
+  lastop_diff l b
+
