inductive_proof/Enable-wins_flag/App.fst
@@ -1,9 +1,5 @@
 module App
 
-open FStar.Seq
-open FStar.Ghost
-module L = FStar.List.Tot
-
 #set-options "--query_stats"
 // the concrete state type
 // It is a pair of counter and flag
@@ -108,7 +104,9 @@ let linearizable_s1_0''_ind (lca s1 s2':st) (last2:op_t)
           (ensures eq (do (v_of s2') last2) (concrete_merge (v_of lca) (v_of s1) (do (v_of s2') last2))) = ()
           
 let linearizable_s1_0_s2_0_base (lca s1 s2:st)
-  : Lemma (requires ops_of s1 == ops_of lca /\ ops_of s2 == ops_of lca)
+  : Lemma (requires (exists l1. v_of s1 == apply_log (v_of lca) l1) /\
+                    (exists l2. v_of s2 == apply_log (v_of lca) l2) /\
+                    ops_of s1 == ops_of lca /\ ops_of s2 == ops_of lca)
         
           (ensures eq (v_of lca) (concrete_merge (v_of lca) (v_of s1) (v_of s2))) = ()
 
