inductive_proof/PN_counter/App.fst
@@ -1,9 +1,5 @@
 module App
 
-open FStar.Seq
-open FStar.Ghost
-module L = FStar.List.Tot
-
 #set-options "--query_stats"
 // the concrete state type
 type concrete_st = int
@@ -94,7 +90,9 @@ let linearizable_s1_0''_ind (lca s1 s2':st) (last2:op_t)
           (ensures eq (do (v_of s2') last2) (concrete_merge (v_of lca) (v_of s1) (do (v_of s2') last2))) = ()
           
 let linearizable_s1_0_s2_0_base (lca s1 s2:st)
-  : Lemma (requires ops_of s1 == ops_of lca /\ ops_of s2 == ops_of lca)
+  : Lemma (requires (exists l1. v_of s1 == apply_log (v_of lca) l1) /\
+                    (exists l2. v_of s2 == apply_log (v_of lca) l2) /\
+                    ops_of s1 == ops_of lca /\ ops_of s2 == ops_of lca)
         
           (ensures eq (v_of lca) (concrete_merge (v_of lca) (v_of s1) (v_of s2))) = ()
 
@@ -157,6 +155,8 @@ let linearizable_gt0_base (lca s1 s2:st) (last1 last2:op_t)
 let linearizable_gt0_ind (lca s1 s2:st) (last1 last2:op_t)
   : Lemma (requires consistent_branches_s2_gt0 lca s1 s2 /\
                     fst last1 <> fst last2 /\
+                    distinct_ops (snoc (ops_of s1) last1) /\
+                    distinct_ops (snoc (ops_of s2) last2) /\
                     (exists l1. (do (v_of s1) last1 == apply_log (v_of lca) l1)) /\
                     (exists l2. (do (v_of s2) last2 == apply_log (v_of lca) l2)) /\
                     (let s2' = inverse_st s2 in
@@ -183,6 +183,8 @@ let linearizable_gt0_ind (lca s1 s2:st) (last1 last2:op_t)
 let linearizable_gt0_ind1 (lca s1 s2:st) (last1 last2:op_t)
   : Lemma (requires consistent_branches_s1_gt0 lca s1 s2 /\
                     fst last1 <> fst last2 /\
+                    distinct_ops (snoc (ops_of s1) last1) /\
+                    distinct_ops (snoc (ops_of s2) last2) /\
                     (exists l1. (do (v_of s1) last1 == apply_log (v_of lca) l1)) /\
                     (exists l2. (do (v_of s2) last2 == apply_log (v_of lca) l2)) /\
                     (let s1' = inverse_st s1 in
